data/predefined/normal_typing.ml
@@ -44,6 +44,8 @@ val tree_mem : 'a tree -> 'a -> bool
 val bst : 'a tree -> bool
 val heap : 'a tree -> bool
 val complete : 'a tree -> bool
+val lower_bound : int tree -> int -> bool
+val upper_bound : int tree -> int -> bool
 
 (* for rbtree *)
 val num_black : 'a rbtree -> int -> bool
