data/subtyping/bst_leaf_rev.ml
@@ -2,15 +2,15 @@ let[@assert] rty1 =
   let d = (0 <= v : [%v: int]) [@over] in
   let lo = (true : [%v: int]) [@over] in
   let hi = (lo < v : [%v: int]) [@over] in
-  (leaf v && d == 0
-   && (not (leaf v)) #==> (lower_bound v lo && upper_bound v hi)
-   && bst v
-   && fun ((n [@exists]) : int) -> depth v n && n <= d
-    : [%v: int tree])
-    [@under]
+  (leaf v && d == 0 : [%v: int tree]) [@under]
 
 let[@assert] rty2 =
   let d = (0 <= v : [%v: int]) [@over] in
   let lo = (true : [%v: int]) [@over] in
   let hi = (lo < v : [%v: int]) [@over] in
-  (leaf v && d == 0 : [%v: int tree]) [@under]
+  (leaf v && d == 0
+   && ((not (leaf v)) #==> (lower_bound v lo && upper_bound v hi))
+   && bst v
+   && fun ((n [@exists]) : int) -> depth v n && n <= d
+    : [%v: int tree])
+    [@under]
