data/subtyping/bst_node_bound_x_min.ml
@@ -3,23 +3,15 @@ let[@assert] rty1 =
   let lo = (true : [%v: int]) [@over] in
   let hi = (lo < v : [%v: int]) [@over] in
   (fun ((lt [@exists]) : int tree) ((rt [@exists]) : int tree)
-       ((d_1 [@exists]) : int) ((d_2 [@exists]) : int) ((x [@exists]) : int) ->
+       ((x [@exists]) : int) ->
      d > 0
      && lo + 1 < hi
      && lo < x && x < hi
-     && 0 <= d - 1
-     && d - 1 >= 0
-     && d - 1 < d
      && ((not (leaf lt)) #==> (lower_bound lt lo))
      && ((not (leaf lt)) #==> (upper_bound lt x))
-     && bst lt
-     && (fun ((n [@exists]) : int) -> depth lt n && n <= d - 1)
-     && 0 <= d_2 && d_2 >= 0 && d_2 < d
-     && d_2 == d - 1
-     && x < hi && bst rt
+     && bst lt && x < hi && bst rt
      && ((not (leaf rt)) #==> (lower_bound rt x))
      && ((not (leaf rt)) #==> (upper_bound rt hi))
-     && (fun ((n [@exists]) : int) -> depth rt n && n <= d_2)
      && root v x && lch v lt && rch v rt
     : [%v: int tree])
     [@under]
@@ -32,11 +24,7 @@ let[@assert] rty2 =
    && ((not (leaf v)) #==> (lower_bound v lo))
    && ((not (leaf v)) #==> (upper_bound v hi))
    && bst v
-   && (not (leaf v))
-   (* && (fun ((x [@exists]) : int) ((lt [@exists]) : int tree) ->
-        root v x && lch v lt && upper_bound lt x) *)
-   (* && (fun ((x [@exists]) : int) ((rt [@exists]) : int tree) ->
-        root v x && rch v rt && lower_bound rt x) *)
+   && not (leaf v)
    && fun ((n [@exists]) : int) -> depth v n && n <= d
     : [%v: int tree])
     [@under]
