data/subtyping/stlc_gen_app_app_tau_rev.ml
@@ -3,36 +3,33 @@ let[@assert] rty1 =
   let num = (v >= 0 : [%v: int]) [@over] in
   let gamma = (true : [%v: stlc_tyctx]) [@over] in
   let tau = (num_arr v num_arr_tau : [%v: stlc_ty]) [@over] in
-  (num > 0 (* && fun ((arg_ty [@exists]) : stlc_ty) ->
-   0 <= num && fun ((num_app_func [@exists]) : int) ->
+  (num > 0
+   && fun ((arg_tau [@exists]) : stlc_ty) ((num_app_func [@exists]) : int) ->
    0 <= num_app_func && num_app_func < num
-   && fun ((b_2 [@exists]) : int) ->
-   0 <= b_2
-   && b_2 == num - num_app_func
-   && fun ((num_app_arg [@exists]) : int) ->
-   0 <= num_app_arg && num_app_arg < b_2
-   && fun ((func_ty [@exists]) : stlc_ty) ((arg_tau [@exists]) : stlc_ty) ->
+   && fun ((func_ty [@exists]) : stlc_ty) ->
    stlc_ty_arr1 func_ty arg_tau
    && stlc_ty_arr2 func_ty tau
    && fun ((num_arr_func_ty [@exists]) : int) ->
    num_arr func_ty num_arr_func_ty
-   && num_arr_func_ty >= 0 && num_app_func >= 0 && num_arr_func_ty >= 0
+      &&
+   num_arr_func_ty >= 0
    && (num_arr_func_ty < num_arr_tau || num_app_func < num)
-   && fun ((x_8 [@exists]) : stlc_ty) ->
-   stlc_ty_arr1 x_8 arg_tau && stlc_ty_arr2 x_8 tau
-   && num_arr x_8 num_arr_func_ty
+   && fun ((x_7 [@exists]) : stlc_ty) ->
+   stlc_ty_arr1 x_7 arg_tau && stlc_ty_arr2 x_7 tau
+   && num_arr x_7 num_arr_func_ty
    && fun ((func [@exists]) : stlc_term) ->
-   (fun ((arg [@exists]) : stlc_term) ((n [@exists]) : int) ->
-     typing gamma func x_8 && num_app func n && n <= num_app_func)
-   && fun ((num_arr_arg_ty [@exists]) : int) ->
-   num_arr arg_tau num_arr_arg_ty
-   && num_arr_arg_ty >= 0 && num_app_arg >= 0 && num_arr_arg_ty >= 0
-   && (num_arr_arg_ty < num_arr_tau || num_app_arg < num)
-   && num_arr arg_tau num_arr_arg_ty
+          typing gamma func x_7 && num_app func num_app_func
+             && fun ((num_arr_arg_ty [@exists]) : int) ->
+   (* num_arr arg_tau num_arr_arg_ty
+      &&*)
+   num_arr_arg_ty >= 0 && fun ((num_2 [@exists]) : int) ->
+   num_2 >= 0 && num_arr_arg_ty >= 0
+   (* && (num_arr_arg_ty < num_arr_tau || num_2 < num) *)
+   && num_2 == num - num_app_func - 1
+   (* && num_arr arg_tau num_arr_arg_ty *)
    && fun ((arg [@exists]) : stlc_term) ->
-   (fun ((n [@exists]) : int) ->
-     typing gamma arg arg_tau && num_app arg n && n <= num_app_arg)
-   && stlc_app1 v func && stlc_app2 v arg *)
+   typing gamma arg arg_tau && num_app arg num_2 &&
+   stlc_app1 v func && stlc_app2 v arg
     : [%v: stlc_term])
     [@under]
 
@@ -41,9 +38,6 @@ let[@assert] rty2 =
   let num = (v >= 0 : [%v: int]) [@over] in
   let gamma = (true : [%v: stlc_tyctx]) [@over] in
   let tau = (num_arr v num_arr_tau : [%v: stlc_ty]) [@over] in
-  (fun ((func [@exists]) : stlc_term) ((arg [@exists]) : stlc_term)
-       ((n [@exists]) : int) ->
-     num > 0 && typing gamma v tau && num_app v n && n <= num
-     && stlc_app1 v func && stlc_app2 v arg
+  (num > 0 && typing gamma v tau && num_app v num && is_app v
     : [%v: stlc_term])
     [@under]
